Add Isabelle to LaTeX makeup and snippets generation to new version

graalir2/Canonicalization.thy
@@ -24,12 +24,12 @@ lemma add_const_nodes:
   assumes yn: "kind g y = ConstantNode yv"
   assumes zn: "kind g z = AddNode x y"
   assumes wn: "kind g w = ConstantNode (xv+yv)"
-  assumes ez: "g m \<turnstile> z (kind g z) \<mapsto> v1"
-  assumes ew: "g m \<turnstile> w (kind g w) \<mapsto> v2"
+  assumes ez: "g m \<turnstile> z (kind g z) \<mapsto> (IntVal v1)"
+  assumes ew: "g m \<turnstile> w (kind g w) \<mapsto> (IntVal v2)"
   shows "v1 = v2"
 proof -
   have zv: "g m \<turnstile> z (kind g z) \<mapsto> IntVal(xv+yv)"
-    using AddNode eval_const_node xn yn zn by auto
+    using AddNode eval_const_node xn yn zn by simp
   have wv: "g m \<turnstile> w (kind g w) \<mapsto> IntVal(xv+yv)"
     using eval_const_node wn by auto
   show ?thesis using det zv wv
@@ -43,11 +43,11 @@ fun create_add_node :: "IRGraph \<Rightarrow> ID \<Rightarrow> ID \<Rightarrow> 
       ConstantNode xv \<Rightarrow> 
         (case kind g y of
           ConstantNode yv \<Rightarrow> ConstantNode (xv+yv) | 
-          _ \<Rightarrow> if xv = 0 then Ref y else AddNode x y
+          _ \<Rightarrow> if xv = 0 then RefNode y else AddNode x y
         ) |
       _ \<Rightarrow> (case kind g y of
             ConstantNode yv \<Rightarrow> 
-              if yv = 0 then Ref x else AddNode x y |
+              if yv = 0 then RefNode x else AddNode x y |
             _ \<Rightarrow> AddNode x y
            )
     )"
@@ -55,32 +55,38 @@ text_raw \<open>}%endsnip\<close>
 
 text_raw \<open>\snip{add_node_create}{\<close>
 lemma add_node_create:
+  assumes xn: "xn = kind g x"
+  assumes yn: "yn = kind g y"
+  assumes xv: "g m \<turnstile> x xn \<mapsto> IntVal(xv)"
+  assumes yv: "g m \<turnstile> y yn \<mapsto> IntVal(yv)"
   assumes det: "\<forall>g m x n v1 v2. 
     (g m \<turnstile> x n \<mapsto> v1) \<and> (g m \<turnstile> x n \<mapsto> v2) \<longrightarrow> v1 = v2"
-  assumes xv: "g m \<turnstile> x (kind g x) \<mapsto> IntVal(xv)"
-  assumes yv: "g m \<turnstile> y (kind g y) \<mapsto> IntVal(yv)"
   shows "(g m \<turnstile> nid (AddNode x y) \<mapsto> IntVal(xv+yv)) \<and>
          (g m \<turnstile> nid (create_add_node g x y) \<mapsto> IntVal(xv+yv))"
 proof -
   have ae: "g m \<turnstile> nid (AddNode x y) \<mapsto> IntVal(xv+yv)"
-    using eval_add_node xv yv by blast
+    using eval_add_node xn yn xv yv by blast
+  have refx: "g m \<turnstile> zx (RefNode x) \<mapsto> IntVal xv"
+    using RefNode xn xv by blast 
+  have refy: "g m \<turnstile> zy (RefNode y) \<mapsto> IntVal yv"
+    using RefNode yn yv by blast 
   have ce: "g m \<turnstile> nid (create_add_node g x y) \<mapsto> IntVal(xv+yv)"
   proof (cases "kind g x  = ConstantNode xvv")
     case xvvn: True
     have xvv: "xvv = xv" 
-      using ConstantNode det xv eval.ConstantNode xvvn by fastforce 
+      using ConstantNode det xn xv eval.ConstantNode xvvn by fastforce 
     thus ?thesis 
     proof (cases "kind g y = ConstantNode yvv")
       case True
       have yvv: "yvv = yv"
-        using ConstantNode det yv eval.ConstantNode True by fastforce
+        using ConstantNode det yn yv eval.ConstantNode True by fastforce
       then show ?thesis
       proof -
         have xvv_yvv: "g m \<turnstile> nid (ConstantNode (xvv+yvv)) \<mapsto> IntVal(xv+yv)"
           by (simp add: ConstantNode xvv yvv) 
         have c_xvv_yvv: "create_add_node g x y = ConstantNode (xvv+yvv)" 
-          apply auto using xvvn True by simp  
-        have cv: "g m \<turnstile> nid (create_add_node g x y) \<mapsto> IntVal(xv+yv)"
+          using xvvn True by simp  
+        have cv1: "g m \<turnstile> nid (create_add_node g x y) \<mapsto> IntVal(xv+yv)"
           using c_xvv_yvv xvv_yvv by simp
         then show ?thesis by blast 
       qed
@@ -88,8 +94,41 @@ proof -
       case False
       then show ?thesis
       proof -
-        have "create_add_node g x y = (if xvv = 0 then Ref y else AddNode x y)"
-          using xvvn False 
+        have cv2: "create_add_node g x y = (if xvv = 0 then RefNode y else AddNode x y)"
+        proof (cases "xvv = 0")
+          case True
+          then show ?thesis 
+            sorry
+        next
+          case False
+          then show ?thesis
+            sorry
+        qed
+        then show ?thesis using cv2 ae xvv yn yv RefNode by auto
+      qed
+    qed
+  next
+    case xnotconst: False
+    thus ?thesis 
+    proof (cases "kind g y = ConstantNode yvv")
+      case True
+      have yvv: "yvv = yv"
+        using ConstantNode True det yn yv eval.ConstantNode by fastforce 
+      have cv3: "create_add_node g x y = (if yvv = 0 then RefNode x else AddNode x y)"
+        using xnotconst True
+        sorry
+      then show ?thesis using cv3 ae yvv xn xv RefNode by auto
+    next 
+      case False
+      have cv4: "create_add_node g x y = AddNode x y"
+        using xnotconst False 
+        sorry
+      thus ?thesis using cv4 ae by simp
+    qed
+  qed
+  thus ?thesis
+    using ae by blast
+qed
 
 text_raw \<open>}%endsnip\<close>
 
