graalir2/gendoc.sh
@@ -1,0 +1,5 @@
+#!/bin/bash
+
+isabelle build -d . -v -c semantics
+
+find output/document -type f -name "*.tex" -exec sed -n '/snip/,/endsnip/p' {} + > "../../papers/cpp-2021/snippets.tex"
